implement cbor_is_equal in Pulse

pulse/share/steel/examples/pulse/dice/cbor/CBOR.Pulse.fst
@@ -1,9 +1,295 @@
 module CBOR.Pulse
+include CBOR.Spec.Constants
 include CBOR.Pulse.Extern
 open Pulse.Lib.Pervasives
 open Pulse.Lib.Stick
 
 module Cbor = CBOR.Spec
+module A = Pulse.Lib.Array
+module SZ = FStar.SizeT
+
+assume val elim_stick0
+  (_: unit)
+  (#hyp #concl: vprop)
+: stt_ghost unit emp_inames
+    ((hyp @==> concl) ** hyp)
+    (fun _ -> concl)
+
+assume val stick_refl0
+    (p: vprop)
+: stt_ghost unit emp_inames
+    (emp)
+    (fun _ -> p @==> p)
+assume
+val stick_consume_l
+    (_: unit)
+    (#p #q #r: vprop)
+: stt_ghost unit emp_inames
+    (p ** ((p ** q) @==> r))
+    (fun _ -> q @==> r)
+
+assume
+val stick_consume_r
+    (_: unit)
+    (#q #p #r: vprop)
+: stt_ghost unit emp_inames
+    (p ** ((q ** p) @==> r))
+    (fun _ -> q @==> r)
+
+assume
+val stick_trans
+    (_: unit)
+    (#p #q #r: vprop)
+: stt_ghost unit emp_inames
+    ((p @==> q) ** (q @==> r))
+    (fun _ -> p @==> r)
+
+assume
+val rewrite_with_implies
+    (p q: vprop)
+: stt_ghost unit emp_inames
+    (p ** pure (p == q))
+    (fun _ -> q ** (q @==> p))
+
+assume
+val stick_weaken_hyp_r
+    (hl hr #hr' #c: vprop)
+: stt_ghost unit emp_inames
+    ((hr' @==> hr) ** ((hl ** hr) @==> c))
+    (fun _ -> (hl ** hr') @==> c)
+
+assume
+val stick_weaken_hyp_l
+    (hl hr #hl' #c: vprop)
+: stt_ghost unit emp_inames
+    ((hl' @==> hl) ** ((hl ** hr) @==> c))
+    (fun _ -> (hl' ** hr) @==> c)
+
+assume Fits_u64 : squash (SZ.fits_u64)
+
+```pulse
+fn rec cbor_is_equal
+  (a1: cbor)
+  (a2: cbor)
+  (#p1: perm)
+  (#p2: perm)
+  (#v1: Ghost.erased Cbor.raw_data_item)
+  (#v2: Ghost.erased Cbor.raw_data_item)
+requires
+    (raw_data_item_match p1 a1 v1 ** raw_data_item_match p2 a2 v2)
+returns res: bool
+ensures
+    (raw_data_item_match p1 a1 v1 ** raw_data_item_match p2 a2 v2 ** pure (
+      (res == true <==> v1 == v2)
+    ))
+{
+    let test = cbor_is_equal_aux a1 a2;
+    match test {
+        CborEqual ->
+        {
+            true
+        }
+        CborNotEqual ->
+        {
+            false
+        }
+        _ ->
+        {
+            let ty1 = cbor_get_major_type a1;
+            let ty2 = cbor_get_major_type a2;
+            if (ty1 <> ty2)
+            {
+                false
+            } else if (ty1 = major_type_uint64 || ty1 = major_type_neg_int64) {
+                let i1 = destr_cbor_int64 a1;
+                let i2 = destr_cbor_int64 a2;
+                (i1.cbor_int_value = i2.cbor_int_value)
+            } else if (ty1 = major_type_simple_value) {
+                let i1 = destr_cbor_simple_value a1;
+                let i2 = destr_cbor_simple_value a2;
+                (i1 = i2)
+            } else if (ty1 = major_type_byte_string || ty1 = major_type_text_string) {
+                let s1 = destr_cbor_string a1;
+                let s2 = destr_cbor_string a2;
+                if (s1.cbor_string_length <> s2.cbor_string_length) {
+                    elim_stick0 ();
+                    elim_stick0 ();
+                    false
+                } else {
+                    A.pts_to_len s1.cbor_string_payload;
+                    A.pts_to_len s2.cbor_string_payload;
+                    let test = A.compare (SZ.uint64_to_sizet s1.cbor_string_length) s1.cbor_string_payload s2.cbor_string_payload;
+                    elim_stick0 ();
+                    elim_stick0 ();
+                    test
+                }
+            } else if (ty1 = major_type_array) {
+                let len1 = cbor_array_length a1;
+                let len2 = cbor_array_length a2;
+                if (len1 <> len2) {
+                    false
+                } else {
+                    let i10 = cbor_array_iterator_init a1;
+                    let i20 = cbor_array_iterator_init a2;
+                    let done0 = cbor_array_iterator_is_done i10;
+                    let mut pi1 = i10;
+                    let mut pi2 = i20;
+                    let mut pdone = done0;
+                    let mut pres = true;
+                    while (
+                        let done = !pdone;
+                        let res = !pres;
+                        (res && not done)
+                    )
+                    invariant cont . exists i1 i2 done res l1 l2 .
+                        pts_to pi1 i1 ** pts_to pi2 i2 ** pts_to pdone done ** pts_to pres res **
+                        cbor_array_iterator_match p1 i1 l1 **
+                        cbor_array_iterator_match p2 i2 l2 **
+                        `@(cbor_array_iterator_match p1 i1 l1 @==> raw_data_item_match p1 a1 v1) **
+                        `@(cbor_array_iterator_match p2 i2 l2 @==> raw_data_item_match p2 a2 v2) **
+                        pure (
+                            List.Tot.length l1 == List.Tot.length l2 /\
+                            (Ghost.reveal (v1 == v2) <==> (res == true /\ l1 == l2)) /\
+                            (res == true ==> done == Nil? l1) /\
+                            cont == (Cons? l1 && res)
+                        )
+                    {
+                        let x1 = cbor_array_iterator_next pi1;
+                        with v1' . assert (raw_data_item_match p1 x1 v1');
+                        let x2 = cbor_array_iterator_next pi2;
+                        with v2' . assert (raw_data_item_match p2 x2 v2');
+                        let test = perform (fun _ -> cbor_is_equal x1 x2 #p1 #p2 #v1' #v2');
+                        with gi1' l1' . assert (pts_to pi1 gi1' ** cbor_array_iterator_match p1 gi1' l1');
+                        with gi2' l2' . assert (pts_to pi2 gi2' ** cbor_array_iterator_match p2 gi2' l2');
+                        stick_consume_l ()
+                            #(raw_data_item_match p1 x1 v1')
+                            #(cbor_array_iterator_match p1 gi1' l1');
+                        stick_consume_l ()
+                            #(raw_data_item_match p2 x2 v2')
+                            #(cbor_array_iterator_match p2 gi2' l2');
+                        stick_trans ()
+                            #(cbor_array_iterator_match p1 gi1' l1');
+                        stick_trans ()
+                            #(cbor_array_iterator_match p2 gi2' l2');
+                        if (test) {
+                            let i1 = !pi1;
+                            rewrite each gi1' as i1;
+                            let done = cbor_array_iterator_is_done i1;
+                            pdone := done
+                        } else {
+                            pres := false
+                        }
+                    };
+                    elim_stick0 ();
+                    elim_stick0 ();
+                    !pres
+                }
+            } else if (ty1 = major_type_tagged) {
+                let tg1 = destr_cbor_tagged a1;
+                let tg2 = destr_cbor_tagged a2;
+                if (tg1.cbor_tagged_tag <> tg2.cbor_tagged_tag) {
+                    elim_stick0 ();
+                    elim_stick0 ();
+                    false
+                } else {
+                    with v1' . assert (raw_data_item_match p1 tg1.cbor_tagged_payload v1');
+                    with v2' . assert (raw_data_item_match p2 tg2.cbor_tagged_payload v2');
+                    let test = perform (fun _ -> cbor_is_equal tg1.cbor_tagged_payload tg2.cbor_tagged_payload #p1 #p2 #v1' #v2');
+                    elim_stick0 ();
+                    elim_stick0 ();
+                    test
+                }
+            } else if (ty1 = major_type_map) {
+                let len1 = cbor_map_length a1;
+                let len2 = cbor_map_length a2;
+                if (len1 <> len2) {
+                    false
+                } else {
+                    let i10 = cbor_map_iterator_init a1;
+                    let i20 = cbor_map_iterator_init a2;
+                    let done0 = cbor_map_iterator_is_done i10;
+                    let mut pi1 = i10;
+                    let mut pi2 = i20;
+                    let mut pdone = done0;
+                    let mut pres = true;
+                    while (
+                        let done = !pdone;
+                        let res = !pres;
+                        (res && not done)
+                    )
+                    invariant cont . exists i1 i2 done res l1 l2 .
+                        pts_to pi1 i1 ** pts_to pi2 i2 ** pts_to pdone done ** pts_to pres res **
+                        cbor_map_iterator_match p1 i1 l1 **
+                        cbor_map_iterator_match p2 i2 l2 **
+                        `@(cbor_map_iterator_match p1 i1 l1 @==> raw_data_item_match p1 a1 v1) **
+                        `@(cbor_map_iterator_match p2 i2 l2 @==> raw_data_item_match p2 a2 v2) **
+                        pure (
+                            List.Tot.length l1 == List.Tot.length l2 /\
+                            (Ghost.reveal (v1 == v2) <==> (res == true /\ l1 == l2)) /\
+                            (res == true ==> done == Nil? l1) /\
+                            cont == (Cons? l1 && res)
+                        )
+                    {
+                        let x1 = cbor_map_iterator_next pi1;
+                        with v1' . assert (raw_data_item_map_entry_match p1 x1 v1');
+                        with gi1' l1' . assert (pts_to pi1 gi1' ** cbor_map_iterator_match p1 gi1' l1');
+                        stick_trans ()
+                            #(raw_data_item_map_entry_match p1 x1 v1' ** cbor_map_iterator_match p1 gi1' l1');
+                        let x2 = cbor_map_iterator_next pi2;
+                        with v2' . assert (raw_data_item_map_entry_match p2 x2 v2');
+                        with gi2' l2' . assert (pts_to pi2 gi2' ** cbor_map_iterator_match p2 gi2' l2');
+                        stick_trans ()
+                            #(raw_data_item_map_entry_match p2 x2 v2' ** cbor_map_iterator_match p2 gi2' l2');
+                        unfold (raw_data_item_map_entry_match p1 x1 v1');
+                        unfold (raw_data_item_map_entry_match p2 x2 v2');
+                        let test = perform (fun _ -> cbor_is_equal (cbor_map_entry_key x1) (cbor_map_entry_key x2) #p1 #p2 #(fstp v1') #(fstp v2'));
+                        if test ensures exists res done . // FIXME: HOW HOW HOW can I frame some things out?
+                            pts_to pi1 gi1' ** pts_to pi2 gi2' ** pts_to pdone done **
+                            raw_data_item_match p1 (cbor_map_entry_key x1) (fstp v1') **
+                            raw_data_item_match p2 (cbor_map_entry_key x2) (fstp v2') **
+                            raw_data_item_match p1 (cbor_map_entry_value x1) (sndp v1') **
+                            raw_data_item_match p2 (cbor_map_entry_value x2) (sndp v2') **
+                            cbor_map_iterator_match p1 gi1' l1' **
+                            cbor_map_iterator_match p2 gi2' l2' **
+                            `@((raw_data_item_map_entry_match p1 x1 v1' ** cbor_map_iterator_match p1 gi1' l1') @==> raw_data_item_match p1 a1 v1) **
+                            `@((raw_data_item_map_entry_match p2 x2 v2' ** cbor_map_iterator_match p2 gi2' l2') @==> raw_data_item_match p2 a2 v2) **
+                            pts_to pres res ** pure (res == true <==> v1' == v2')
+                        {
+                            let test = perform (fun _ -> cbor_is_equal (cbor_map_entry_value x1) (cbor_map_entry_value x2) #p1 #p2 #(sndp v1') #(sndp v2'));
+                            pres := test;
+                        } else {
+                            pres := false;
+                        };
+                        fold (raw_data_item_map_entry_match p1 x1 v1');
+                        fold (raw_data_item_map_entry_match p2 x2 v2');
+                        stick_consume_l ()
+                            #(raw_data_item_map_entry_match p1 x1 v1')
+                            #(cbor_map_iterator_match p1 gi1' l1');
+                        stick_consume_l ()
+                            #(raw_data_item_map_entry_match p2 x2 v2')
+                            #(cbor_map_iterator_match p2 gi2' l2');
+                        let res = !pres;
+                        if (res) {
+                            let i1 = !pi1;
+                            rewrite each gi1' as i1;
+                            let done = cbor_map_iterator_is_done i1;
+                            pdone := done
+                        }
+                    };
+                    elim_stick0 ();
+                    elim_stick0 ();
+                    !pres
+                }
+            } else {
+                // unreachable
+                let unused : squash False = ();
+                false
+            }
+        }
+    }
+}
+
+```
 
 noeq
 type cbor_map_get_t =
@@ -84,20 +370,6 @@ let cbor_map_get_invariant
           list_ghost_assoc (Ghost.reveal vkey) l
     )
 
-assume val elim_stick0
-  (_: unit)
-  (#hyp #concl: vprop)
-: stt_ghost unit emp_inames
-    ((hyp @==> concl) ** hyp)
-    (fun _ -> concl)
-
-assume val stick_refl0
-    (p: vprop)
-: stt_ghost unit emp_inames
-    (emp)
-    (fun _ -> p @==> p)
-
-
 ```pulse
 ghost
 fn cbor_map_get_invariant_end
@@ -142,50 +414,6 @@ ensures
     }
 }
 ```
-assume
-val stick_consume_l
-    (_: unit)
-    (#p #q #r: vprop)
-: stt_ghost unit emp_inames
-    (p ** ((p ** q) @==> r))
-    (fun _ -> q @==> r)
-
-assume
-val stick_consume_r
-    (_: unit)
-    (#q #p #r: vprop)
-: stt_ghost unit emp_inames
-    (p ** ((q ** p) @==> r))
-    (fun _ -> q @==> r)
-
-assume
-val stick_trans
-    (_: unit)
-    (#p #q #r: vprop)
-: stt_ghost unit emp_inames
-    ((p @==> q) ** (q @==> r))
-    (fun _ -> p @==> r)
-
-assume
-val rewrite_with_implies
-    (p q: vprop)
-: stt_ghost unit emp_inames
-    (p ** pure (p == q))
-    (fun _ -> q ** (q @==> p))
-
-assume
-val stick_weaken_hyp_r
-    (hl hr #hr' #c: vprop)
-: stt_ghost unit emp_inames
-    ((hr' @==> hr) ** ((hl ** hr) @==> c))
-    (fun _ -> (hl ** hr') @==> c)
-
-assume
-val stick_weaken_hyp_l
-    (hl hr #hl' #c: vprop)
-: stt_ghost unit emp_inames
-    ((hl' @==> hl) ** ((hl ** hr) @==> c))
-    (fun _ -> (hl' ** hr) @==> c)
 
 ```pulse
 fn cbor_map_get
@@ -197,8 +425,7 @@ fn cbor_map_get
   (#vmap: Ghost.erased Cbor.raw_data_item)
 requires
     (raw_data_item_match pkey key vkey ** raw_data_item_match pmap map vmap ** pure (
-      Cbor.Map? vmap /\
-      (~ (Cbor.Tagged? vkey \/ Cbor.Array? vkey \/ Cbor.Map? vkey))
+      Cbor.Map? vmap
     ))
 returns res: cbor_map_get_t
 ensures
